tests/elab/compile_borrowed_reset_jp.lean
@@ -86,7 +86,6 @@ def testWithoutAnnotation (n : Nat) (p q : Prod Nat Nat) : Prod Nat Nat :=
 trace: [Compiler.inferBorrow] own _x.28: result of ctor call _x.28
 [Compiler.inferBorrow] own _x.30: result of ctor call _x.30
 [Compiler.inferBorrow] own n: argument to constructor call _x.30
-[Compiler.inferBorrow] own _x.29: result of function call _x.29
 [Compiler.inferBorrow] size: 2
     def testArrayWithAnnotation._closed_0 : obj :=
       let _x.1 := 0;
@@ -112,7 +111,6 @@ trace: [Compiler.inferBorrow] own _x.28: used in reset reuse _x.28
 [Compiler.inferBorrow] own n: argument to constructor call _x.28
 [Compiler.inferBorrow] own pair: used in reset reuse _x.29
 [Compiler.inferBorrow] own snd: fwd projection propagation snd
-[Compiler.inferBorrow] own _x.27: result of function call _x.27
 [Compiler.inferBorrow] size: 5
     def testArrayWithoutAnnotation n @&ps : obj :=
       let _x.1 := testArrayWithAnnotation._closed_0;
